Further simplified code for #186

examples/bug-reports/bug186.fst
@@ -1,13 +1,13 @@
 module Bug186
 
 type valid : int -> Type =
-  | VForall     : #p:(int -> Tot int) -> (* non-inferrable *)
-                  f: (x:int -> Tot (valid (p x))) ->
+  | VForall     : p:(int -> Tot int) ->
+                  f: valid (p 67) ->
                   valid 42
 
 val hoare_consequence : valid 42 -> Tot unit
 let hoare_consequence v =
-  let VForall #p fpp' = v in (* #p here doesn't change anything *)
+  let VForall p v' = v in
 (*  ignore (fpp' 75) -- this causes bogus "patterns are incomplete" *)
-  assert (is_VForall (fpp' 75))
+  assert (is_VForall (* this solves it: #(p 67) *) v')
     (* BUG: this makes F* explode: Impossible: Typ_unknown *)
